\documentclass{amsart}
\usepackage[ocgcolorlinks,linktoc=all]{hyperref}
\usepackage{cancel}
\hypersetup{citecolor=blue,linkcolor=red}
\newtheorem{theorem}{Theorem}
\newtheorem*{thmA}{Theorem}
\newtheorem*{thmB}{Theorem}
\newtheorem*{rem}{Remark}
\newtheorem*{thmmain}{Theorem}
\newtheorem{lemma}[theorem]{Lemma}
\newtheorem{proposition}[theorem]{Proposition}
\newtheorem*{propmain}{Proposition}
\newtheorem{corollary}[theorem]{Corollary}
\theoremstyle{definition}
\newtheorem{definition}[theorem]{Definition}
\newtheorem{example}[theorem]{Example}
\newtheorem{xca}[theorem]{Exercise}

\theoremstyle{remark}
\newtheorem{remark}[theorem]{Remark}

\newcommand{\abs}[1]{\lvert#1\rvert}
\newcommand{\ip}[2]{\ensuremath{\langle{#1},{#2}\rangle}}

\DeclareMathOperator{\grad}{grad}
\DeclareMathOperator{\Rm}{Rm}
\DeclareMathOperator{\Tr}{Tr}
\DeclareMathOperator{\hess}{Hess}
\DeclareMathOperator{\ric}{Ric}
\DeclareMathOperator{\diff}{K}
\DeclareMathOperator{\D}{D}
\DeclareMathOperator{\RR}{\mathbb{R}}


\numberwithin{equation}{section}

\newcommand{\blankbox}[2]{%
  \parbox{\columnwidth}{\centering
    \setlength{\fboxsep}{0pt}%
    \fbox{\raisebox{0pt}[#2]{\hspace{#1}}}%
  }%
}

\begin{document}

\title[]
 {}

\curraddr{}
\email{}
\date{\today}

\dedicatory{}
\subjclass[2010]{}
\keywords{}

\begin{abstract}

\end{abstract}

\maketitle
Let $M^n$ be an $n$-dimensional smooth submanifold of $(N^{n+1},\ip{}{})$ given by an embedding $F_0.$ A one-parameter family of immersions $F\colon M^n\times [0,T)\to (N^{n+1},\ip{}{})$ is said to be a solution of the $f$-curvature flow if
\begin{align}
\partial_tF = \xi,\quad F(\cdot, 0) = F_0(\cdot).
\end{align}
Here $\xi $ is a smooth transverse inward-pointing vector field defined by
\begin{align}
\xi := -F_{\ast}\grad_h f + f\nu,
\end{align}
where $f$ is a smooth, positive, strictly increasing and symmetric function of the principle curvatures, $\nu$ is a smooth inner unit normal vector field, and $\grad_h f$ is the gradient of $f$ with respect to the second fundamental $h$ induced by $\nu,$ namely
\[
h(X, \grad_h f) = X(f)
\]
for all vectors $X$ tangent to $M$. In what follows, for convenience, we set $W := -\grad_h f$ so that $\xi = F_{\ast} W + f \nu$.


\section{structure equations}

We make use of the theory of affine immersions as described in \cite{MR1311248}.

Let $\bar{g}$ be the induced metric by the immersion. The Gauss formula is given by
\begin{align}\label{gauss equ}
\D_YF_{\ast}(X)=F_{\ast}(\bar{\nabla}_YX)+h(X,Y)\nu.
\end{align}
Define the non-degenerate metric, referred to here as the \emph{affine metric},
\begin{align}
g(X,Y):=\frac{h(X,Y)}{ f }.
\end{align}
Note that
\begin{align*}
\D_X \xi &= \D_X (F_{\ast}(W) + f \nu) \\
&= \D_X F_{\ast}(W) + X(f)\nu + f \D_X \nu \\
&= F_{\ast}(\bar{\nabla}_X W) - h(X, \grad_h f) \nu + X(f) \nu + f \D_X \nu \\
&= F_{\ast} (\bar{\nabla}_X W) + f \D_X \nu,
\end{align*}
which is tangential since $\nu$ has unit length. Thus, we may define an endomorphism of $TM$, the \emph{affine shape operator} $A$ with respect to $\xi$, by
\begin{align}
\D_X\xi := -F_{\ast}(A(X))
\end{align}
for $X\in TM$. Equivalently,
\[
A(X) =- \bar{\nabla}_X W - f F_{\ast}^{-1} \D_X \nu.
\]
We also have the \emph{affine second fundamental form}, a tensor of type $(0, 2)$, by
\[
B(X, Y) = g(A(X), Y).
\]
In general, the presence of ambient curvature $\widehat{\Rm}$ implies that $A$ is not self-adjoint with respect to $g$ (see \eqref{eq:structure2} below), and hence $B$ is not symmetric. For this reason, we typically will not use $B$, preferring $g(A(X), Y)$ emphasising the lack of symmetry. We only mention $B$ here to emphasise the lack of symmetry, compared with the usual second fundamental form, $\bar{g}(-\D_{\nu} X, Y)$ which is symmetric, and the Weingarten map $-\D_{\nu} X$ which is thus self-adjoint with respect to $\bar{g}$.

The vector field $\xi$ induces a torsion free connection $\tilde{\nabla}$:
\begin{align}\label{gauss equ2}
\D_YF_{\ast}(X)=F_{\ast}(\tilde{\nabla}_YX)+g(X,Y)\xi.
\end{align}
This connection is well defined (i.e. $F_{\ast}(\tilde{\nabla}_Y X)$ is tangent to $F(M)$) since for all $X,Y\in TM$ we have
\begin{align}
F_{\ast}(\tilde{\nabla}_Y X) &= F_{\ast}(\bar{\nabla}_Y X) + h(X, Y) \nu - g(X, Y) (F_{\ast}(W) + f \nu) \\
&= F_{\ast}(\bar{\nabla}_YX)-g(X,Y)F_{\ast}(W) \nonumber.
\end{align}
In other words, $\tilde{\nabla}_Y X$ is the uniquely determined tangential component of $D_Y F_{\ast} X$ in the splitting $F^{\ast} TN \simeq TM \oplus \RR \xi$ where $\RR\xi$ denotes the line bundle over $M$ determined by $\xi$ and $F^{\ast} TN$ denotes the pull-back bundle of $TN$ by $F$.

The connection $\tilde{\nabla}$ is not necessarily the Levi-Civita connection for $g$. Let $\nabla$ be the Levi-Civita connection for $g$; that is $\nabla$ is the unique torsion free connection satisfying $\nabla g=0.$ Define the difference tensor
\begin{equation}
\label{eq:difftensor}
\diff_YX := \tilde{\nabla}_{Y}X - \nabla_{Y}X.
\end{equation}
Since both $\tilde{\nabla}$ and $\nabla$ are torsion free, we have $\diff$ is symmetric: $\diff_YX = \diff_XY.$

From (\ref{gauss equ2}) we get,
\begin{align}\label{gauss equ3}
\hess F(X,Y):=\D_YF_{\ast}(X)-F_{\ast}(\nabla_YX) = F_{\ast}(\diff_YX) + g(X,Y)\xi.
\end{align}

Let us recall the \emph{structure equations} of an affine immersion (see the proof of \cite[Section II, Theorem 2.1]{MR1311248} adjusted to include the ambient curvature $\widehat{Rm}$ or \cite[p. 197 equations (N1.6)--(N1.9)]{MR1311248} in the codimension one case):

\begin{align}
\label{eq:structure1}
\widehat{Rm} (X, Y) Z =& Rm(X, Y) Z + g(X, Z) A Y - g(Y, Z)A X \\
&+ \left[(\tilde{\nabla}_X g) (Y, Z) - (\tilde{\nabla}_Y g)( X, Z)\right] \xi \nonumber,\\
\label{eq:structure2}
\widehat{Rm} (X, Y) \xi &= (\tilde{\nabla}_Y A) X - (\tilde{\nabla}_X A) Y + \left[g(AX, Y) - g(X, AY)\right]\xi.
\end{align}

The \emph{cubic tensor} is defined by
\begin{align}
C(X,Y,Z) = (\tilde{\nabla}_X g) (Y,Z).
\end{align}

We have the following useful lemma for $C$ (see also \cite[Section II, Proposition 4.1]{MR1311248}):

\begin{lemma}
\[
C(X, Y, Z) =  -2g(\diff_Z Y, X) + \left[\widehat{Rm}(X, Y)Z + \widehat{Rm}(X, Z)Y\right]^{\xi}.
\]
\end{lemma}

\begin{proof}
First, since $g$ is symmetric, $C(X, Y, Z) = C(X, Z, Y)$:
\[
\begin{split}
C(X, Y, Z) - C(X, Z, Y) &= (\tilde{\nabla}_X g) (Y, Z) - (\tilde{\nabla}_X g) (Z, Y) \\
&= \tilde{\nabla}_X \left[g(Y, Z) - g(Z, Y)\right] \\
&\quad - g(\tilde{\nabla}_X Y, Z) - g(Y, \tilde{\nabla}_X Z) + g(\tilde{\nabla}_X Z, Y) + g(Z, \tilde{\nabla}_X Y) \\
&= 0.
\end{split}
\]

But if $\widehat{Rm} \ne 0$, $C$ may not be symmetric in the first two slots: using the structure equations,
\[
C(X, Y, Z) = C(Y, X, Z) + [\widehat{Rm}(X, Y)Z]^{\xi},
\]
where the superscript $\xi$ denotes the $\xi$ component in the splitting, $F^{\ast} TN \simeq TM \oplus \RR \xi$. Applying the structure equation to $C(Y, X, Z) = C(Y, Z, X)$, we obtain,
\begin{equation}
\label{eq:cubic_permutation1}
C(X, Y, Z) = C(Z, Y, X) + \left[\widehat{Rm}(Y, Z) X + \widehat{Rm}(X, Y) Z\right]^{\xi}.
\end{equation}
On the other hand, since $\diff_X \varphi = (\tilde{\nabla}_X - \nabla_X) \varphi = 0$ for any smooth function $\varphi$, applying $\diff_X$ to $g$ as a derivation gives,
\[
(\diff_X g) (Y, Z) = \diff_X (g(Y, Z)) - g(\diff_X Y, Z) - g(Y, \diff_X Z) = -g(\diff_X Y, Z) - g(Y, \diff_X Z).
\]
Now using $\nabla g \equiv 0$, gives
\begin{equation}
\label{eq:cubic_derivation_identity}
C(X, Y, Z) = (\tilde{\nabla}_X g) (Y, Z) = (\diff_X g) (Y, Z) + (\nabla_X g) (Y, Z) = -g(\diff_X Y, Z) - g(Y, \diff_X Z).
\end{equation}

Thus from \eqref{eq:cubic_permutation1}, \eqref{eq:cubic_derivation_identity} we obtain,
\begin{equation}
\label{eq:cubic_identity}
\begin{split} 
-g(\diff_X Y, Z) - g(Y, \diff_X Z) &= C(Z, Y, X) + \left[\widehat{Rm}(Y, Z) X + \widehat{Rm}(X, Y)Z\right]^\xi \\
&= -g(\diff_Z Y, X) - g(Y, \diff_Z X) + \left[\widehat{Rm}(Y, Z) X + \widehat{Rm}(X, Y)Z\right]^\xi
\end{split}
\end{equation}
Since $\diff_X Z = \diff_Z X$ this yields,
\[
-g(\diff_X Y, Z) = - g(\diff_Z Y, X) + \left[\widehat{Rm}(Y, Z) X + \widehat{Rm}(X, Y)Z\right]^\xi
\]
When applied to $g(\diff_X Z, Y)$ we obtain
\[
-g(\diff_Z X, Y) = - g(\diff_X Z, Y) = - g(\diff_Y Z, X) + \left[\widehat{Rm}(Z, Y) X + \widehat{Rm}(X, Z)Y\right]^\xi
\]
Finally, upon substitution of this identity into equation \eqref{eq:cubic_identity} we complete the proof with,
\begin{equation}
\begin{split}
C(X, Y, Z) &= -g(\diff_Z Y, X) - g(\diff_Z X, Y) + \left[\widehat{Rm}(Y, Z) X + \widehat{Rm}(X, Y)Z\right]^\xi \\
&= -g(\diff_Z Y, X) - g(\diff_Y Z, X) \\
&\quad + \left[\widehat{Rm}(Y, Z) X + \widehat{Rm}(X, Y)Z + \widehat{Rm}(Z, Y) X + \widehat{Rm}(X, Z)Y\right]^\xi \\
&= - 2g(\diff_Y Z, X) + \left[\widehat{Rm}(X, Y)Z + \widehat{Rm}(X, Z)Y\right]^{\xi}
\end{split}
\end{equation}
where we used the first anti-symmetry of $\widehat{Rm}$ in the last line.
\end{proof}

The second covariant derivatives of $ \xi$ is given by
\begin{align}
\hess\xi(X,Y)&=\D_Y\D_X\xi-\D_{\nabla_YX}\xi\\
&=-\D_YF_{\ast}(AX)+F_{\ast}(A\nabla_YX)\nonumber\\
&=-F_{\ast}(\tilde{\nabla}_{Y}AX)-g(A X,Y)\xi+F_{\ast}(A\nabla_YX)\nonumber\\
&=-F_{\ast}(\nabla_{Y}AX)-F_{\ast}(\diff_{Y}AX)-g(A X,Y)\xi+F_{\ast}(A\nabla_YX)\nonumber\\
&=-F_{\ast}((\nabla_Y A)X)-F_{\ast}(\diff_{Y}AX)-g(A X,Y)\xi.\nonumber
\end{align}

On the other hand, we see that if $\widehat{\Rm}$ does not vanish, then $\hess \xi$ is not symmetric:
\begin{align}
\widehat{Rm}(X,Y)\xi&=\D^2_{X,Y}\xi-\D^2_{Y,X}\xi\\
&=\hess\xi(X,Y)-\hess\xi(Y,X)-\D_{\D_YX-\D_XY}\xi-\D_{\nabla_XY-\nabla_YX}\xi\nonumber\\
&=\hess\xi(X,Y)-\hess\xi(Y,X).\nonumber
\end{align}

\section{evolution equations}

Perhaps the most important aspect of our approach is the following lemma, exhibiting crucial properties of our chosen parametrisation.

\begin{lemma}
\begin{align}
\D_t \nu & = 0, \\
\D_t \bar{g} &= 0.
\end{align}
\end{lemma}

\begin{proof}
As $\ip{\nu}{\nu} = 1$, $\D_{\xi} \nu$ is tangential, and for any tangent vector $X$,
\[
\begin{split}
\ip{\D_{\xi} \nu}{F_{\ast} X} &= D_{\xi} \ip{\nu}{F_{\ast}X} - \ip{\nu}{D_{\xi} F_{\ast} X} \\
&= -\ip{\nu}{\D_{X}\xi} \\
&= \ip{\nu}{A(X)} = 0.
\end{split}
\]

For the metric,
\[
\begin{split}
\left(\D_t \bar{g}\right) (X, Y) &= \D_t (\bar{g}(X, Y)) - \bar{g}(\D_t X, Y) - \bar{g}(X, \D_t Y) \\
&= \D_t (\bar{g}(X, Y)) + \bar{g}(A(X), Y) + \bar{g}(X, A(Y)).
\end{split}
\]
On the other hand,
\[
\begin{split}
\D_t (\bar{g}(X, Y)) &= \D_t \ip{F_{\ast} X}{F_{\ast} Y} \\
&= -\ip{F_{\ast} A(X)}{F_{\ast} Y} - \ip{F_{\ast} X}{F_{\ast} A(Y)}
\end{split}
\]
and the result follows since $\bar{g} = F^{\ast} \ip{}{}$.
\end{proof}

The next lemma contains other basic evolution equations. It will be convenient at this stage to express these equations in terms of $u = \partial_t \ln f$.
\begin{lemma}
\begin{align*}
(\D_t h) (X, Y) &= f g(X, A(Y)) + \ip{\widehat{\Rm}(\xi, X) Y}{\nu} =  f g(A(X), Y) + \ip{\widehat{\Rm}(\xi, Y) X}{\nu}, \\
(\D_t g) (X, Y) &= g(X, A(Y)) - u g(X, Y) + \frac{1}{f} \ip{\widehat{\Rm}(\xi, X) Y}{\nu}, \\
\D_t \grad_h f &= \grad_h \D_t f + R(\grad_h f) = f \grad_h u + u \grad_h f + R(\grad_h f) \\
\intertext{where $h(R({\grad_h f}), X) = \ip{\widehat{\Rm}(\xi, \grad_h f) \nu}{X}$ for any vector field $X$,}
\D_t \xi &= u\xi - f\grad_h u - R(\grad_h f), \\
(\D_t A)(X) &= A^2(X) + u A(X) + \tilde{\nabla}_X (f\grad_h u) + \widehat{\Rm} (\xi, X) \xi + \D_X (R(\grad_h f)).
\end{align*}
\end{lemma}

\begin{proof}
Using $h(X,Y) = \ip{\D_Y X}{\nu} = -\ip{X}{D_Y \nu}$ and $\D_t\nu = 0$, we calculate
\[
\begin{split}
(\D_t h) (X, Y) &= \D_t (h(X, Y)) - h(\D_t X, Y) - h(X, D_t Y) \\
&= \ip{\D_t \D_Y X}{\nu} + f g(A(X), Y) + f g(X, A(Y)) \\
&= \ip{\D_Y \D_{\xi} X}{\nu} + \ip{\widehat{\Rm}(\xi, X) Y}{\nu} + f g(A(X), Y) + f g(X, A(Y))\\
&= \D_Y \ip{\D_{\xi} X}{\nu} - \ip{\D_{\xi} X}{D_Y \nu} + f g(A(X), Y) + f g(X, A(Y)) + \ip{\widehat{\Rm}(\xi, X) Y}{\nu} \\
&= - h(A(X), Y) + f g(A(X), Y) + f g(X, A(Y)) + \ip{\widehat{\Rm}(\xi, X) Y}{\nu} \\
&= fg(X, A(Y)) + \ip{\widehat{\Rm}(\xi, X) Y}{\nu},
\end{split}
\]
giving the first expression for $\D_t h$. The second follows from the symmetry of $\D_t h$.

The metric now follows easily,
\[
\begin{split}
(\D_t g) (X, Y) &= -\frac{1}{f^2} (\D_t f) h(X, Y) + \frac{1}{f} (\D_t h) (X, Y) \\
&= -u g(X, Y) + g(X, A(Y)) + \frac{1}{f} \ip{\widehat{\Rm}(\xi, X) Y}{\nu}.
\end{split}
\]

To compute $\D_t \grad_h f$, we use the defining equation, $h(\grad_h f, X) = X(f) = \D_X f$ to compute,
\[
\begin{split}
h(\grad_h \D_t f, X) &= \D_X \D_t f = \D_t \D_X f \\
&=  \D_t (h(\grad_h f, X)) \\
&= (\D_t h) (\grad_h f, X)) + h(\D_t \grad_h f, X) + h(\grad_h f, \D_t X) \\
&= fg (\grad_h f, A(X)) + \ip{\widehat{\Rm}(\xi, \grad_h f)X}{\nu} \\
&\quad + h(\D_t \grad_h f, X) - h(\grad_h f, A(X)) \\
&= h(\D_t \grad_h f, X) - \ip{\widehat{\Rm}(\xi, \grad_h f)\nu}{X}.
\end{split}
\]
Rearranging gives,
\[
h(\D_t \grad_h f - \grad_h \D_t f, X) = \ip{\widehat{\Rm}(\xi, \grad_h f) \nu}{X}.
\]
Since this is true for any $X$, the desired result follows. The second expression for $\D_t \grad_h f$ is obtained from,
\[
\grad_h \D_t f = \grad_h (f u) = f \grad_h u + u \grad_h f.
\]

The evolution of $\xi$ follows readily, using this second expression and $\D_t f = f u$:
\[
\begin{split}
\D_t \xi &= \D_t (-\grad_h f + f \nu) \\
& = -f \grad_h u - u \grad_h f + (\D_t f) \nu - R(\grad_h f) \\
&= u\xi - f\grad_h u - R(\grad_h f).
\end{split}
\]

Finally, for any $X$,
\[
\begin{split}
(\D_t A)(X) &= \D_t (A(X)) - A(\D_t X) \\
&= - \D_t \D_X \xi + A^2(X) \\
&= -\D_X \D_t \xi + A^2(X) + \widehat{\Rm} (\xi, X) \xi \\
&= -\D_X \left(u\xi - f\grad_h u - R(\grad_h f)\right) + A^2(X) + \widehat{\Rm} (\xi, X) \xi \\
&= A^2(X) + u A(X) -(\D_X u)\xi + \D_X (f\grad_h u) + \widehat{\Rm} (\xi, X) \xi + \D_X (R(\grad_h f)).
\end{split}
\]
To finish, we observe that by equation \eqref{gauss equ2} defining $\tilde{\nabla}$ we have,
\[
\begin{split}
-(\D_X u)\xi + \D_X (f\grad_h u) &= -(\D_X u)\xi + \tilde{\nabla}_X (f\grad_h u) + g(f \grad_h u, X) \xi \\
&= \tilde{\nabla}_X (f\grad_h u) + (-X(u) + h(\grad_h u, X))\xi \\
&= \tilde{\nabla}_X (f\grad_h u).
\end{split}
\]
\end{proof}

Next, we compute the evolution of $\xi = -\grad_h f + f \nu$. This is somewhat more involved than the previous lemma.

\begin{lemma}
\[
\D_{\xi} \xi = \left[1 -\frac{p}{|p|}\right] A(\grad_h f) +
|p|\mathcal{H}\xi - |p| f \grad_h\mathcal{H} + R
\]
where $R$ satisfies,
\[
\begin{split}
g(R - |p| \Tr (\widehat{Rm}(\xi,\cdot,\cdot,\nu))) \nu, X) &= |p|\frac{1}{f} g(\Tr \left(\widehat{Rm}(\xi, \cdot, \cdot, \nu)\right)\grad_h f, X) - |p| g(\grad_h \Tr \left(\widehat{Rm}(\xi, \cdot, \cdot, \nu)\right), X) \\
&\quad + \frac{p}{|p|f} \left[\langle \widehat{Rm}(\xi,\grad_h f)X,\nu\rangle -
\Tr (\widehat{Rm}(\xi,\cdot,\cdot,\nu))g(\grad_h f, X)\right] \\
&\quad  -\frac{p}{|p|} \left[\widehat{Rm}(X, \grad_h f)\xi\right]^{\xi}.
\end{split}
\]
\end{lemma}

\begin{proof}
\begin{equation}
\label{eq:dt_transverse_productrule}
\begin{split}
\D_{\xi}\xi &= -\D_{\xi} \left(\grad_h f\right) + (\partial_t f) \nu \\
&= -\D_{\xi}\left(\grad_h f\right) + |p|(f\mathcal{H}+\Tr (\widehat{Rm}(\xi,\cdot,\cdot,\nu))) \nu
\end{split}
\end{equation}
Now we use the defining equation for $\grad_h f$,
\[
X(\ln f) = \frac{1}{f} h(\grad_h f, X) = g(\grad_h f, X)
\]
We then compute
\[
\begin{split}
\D_{\xi} \left(X(\ln f)\right) &= \D_{\xi} \left[g(\grad_h f, X)\right] \\
&= (\D_{\xi} g) (\grad_h f, X) + g(\D_{\xi} \grad_h f, X) + g(\grad_h f,  \D_{\xi} X).
\end{split}
\]
Rearranging gives,
\begin{equation}
\label{eq:dt_transversegradient_structure}
\begin{split}
-g(\D_{\xi} \grad_h f, X) &= -\D_{\xi} \left(X(\ln f)\right) + (\D_{\xi} g) ((\grad_h f, X) + g(\grad_h,  \D_{\xi} X) \\
&= -X(\partial_t \ln f) + (\D_{\xi} g) ((\grad_h f, X) - g(\grad_h f,  A(X))
\end{split}
\end{equation}

The first term of equation \eqref{eq:dt_transversegradient_structure} is,
\[
\begin{split}
-X(\partial_t \ln f) &= -X\left[|p|(\mathcal{H} + \frac{1}{f} \Tr (\widehat{Rm}(\xi,\cdot,\cdot,\nu)))\right] \\
&= -|p| h(\grad_h \mathcal{H}, X) \\
&\quad + |p|\frac{1}{f^2} h(\Tr \left(\widehat{Rm}(\xi, \cdot, \cdot, \nu)\right)\grad_h f, X) - \frac{|p|}{f} h(\grad_h \Tr \left(\widehat{Rm}(\xi, \cdot, \cdot, \nu)\right), X) \\
&= -|p| fg(\grad_h \mathcal{H}, X) \\
&\quad + |p|\frac{1}{f} g(\Tr \left(\widehat{Rm}(\xi, \cdot, \cdot, \nu)\right)\grad_h f, X) - |p| g(\grad_h \Tr \left(\widehat{Rm}(\xi, \cdot, \cdot, \nu)\right), X),
\end{split}
\]
Using the symmetry of $\D_{\xi}$, the late two terms of equation \eqref{eq:dt_transversegradient_structure} are
\[
\begin{split}
(\D_{\xi} g) (X, \grad_h f) - g(\grad_h f, A(X)) &= \left(1 -\frac{p}{|p|}\right) g(\grad_h f, A(X)) -
|p|\mathcal{H} g(\grad_h f, X) \\
&\quad + \frac{p}{|p|f} \left[\langle \widehat{Rm}(\xi,\grad_h f)X,\nu\rangle -
\Tr (\widehat{Rm}(\xi,\cdot,\cdot,\nu))g(X,\grad_h f)\right] \\
&\quad - \left[\widehat{Rm}(X, \grad_h f)\xi\right]^{\xi} \\
&= g\left(\left[1 -\frac{p}{|p|}\right] A(\grad_h f) -
|p|\mathcal{H} \grad_h f, X\right) \\
&\quad + \frac{p}{|p|f} \left[\langle \widehat{Rm}(\xi,\grad_h f)X,\nu\rangle -
\Tr (\widehat{Rm}(\xi,\cdot,\cdot,\nu))g(\grad_h f, X)\right] \\
&\quad  -\frac{p}{|p|} \left[\widehat{Rm}(X, \grad_h f)\xi\right]^{\xi}
\end{split}
\]
upon using the structure equation \eqref{eq:structure2} to get the second line.

Therefore we may rewrite \eqref{eq:dt_transversegradient_structure} as
\begin{equation}
\label{eq:dt_transversegradient_structure2}
\begin{split}
-g(\D_{\xi} \grad_h \ln f, X) &= -|p| fg(\grad_h \mathcal{H}, X) \\
&\quad + |p|\frac{1}{f} g(\Tr \left(\widehat{Rm}(\xi, \cdot, \cdot, \nu)\right)\grad_h f, X) - |p| g(\grad_h \Tr \left(\widehat{Rm}(\xi, \cdot, \cdot, \nu)\right), X) \\
&\quad + g\left(\left[1 -\frac{p}{|p|}\right] A(\grad_h f) -
|p|\mathcal{H} \grad_h f, X\right) \\
&\quad + \frac{p}{|p|f} \left[\langle \widehat{Rm}(\xi,\grad_h f)X,\nu\rangle -
\Tr (\widehat{Rm}(\xi,\cdot,\cdot,\nu))g(\grad_h f, X)\right] \\
&\quad  -\frac{p}{|p|} \left[\widehat{Rm}(X, \grad_h f)\xi\right]^{\xi} \\
&= g\left(\left[1 -\frac{p}{|p|}\right] A(\grad_h f) -
|p|\mathcal{H} \grad_h f -|p| f \grad_h \mathcal{H}, X\right) \\
&\quad + |p|\frac{1}{f} g(\Tr \left(\widehat{Rm}(\xi, \cdot, \cdot, \nu)\right)\grad_h f, X) - |p| g(\grad_h \Tr \left(\widehat{Rm}(\xi, \cdot, \cdot, \nu)\right), X) \\
&\quad + \frac{p}{|p|f} \left[\langle \widehat{Rm}(\xi,\grad_h f)X,\nu\rangle -
\Tr (\widehat{Rm}(\xi,\cdot,\cdot,\nu))g(\grad_h f, X)\right] \\
&\quad  -\frac{p}{|p|} \left[\widehat{Rm}(X, \grad_h f)\xi\right]^{\xi}
\end{split}
\end{equation}

Since this is true for any $X$, this uniquely determines $-\D_{\xi} \grad_h f$, and upon substitution into equation \eqref{eq:dt_transverse_productrule2} we obtain
\begin{equation}
\label{eq:dt_transverse_productrule2}
\begin{split}
\D_{\xi}\xi &= -\D_{\xi}\left(\grad_h f\right) + |p|(f\mathcal{H} + \Tr (\widehat{Rm}(\xi,\cdot,\cdot,\nu))) \nu \\
&= \left[1 -\frac{p}{|p|}\right] A(\grad_h f) +
|p|\left[f \mathcal{H} - \mathcal{H} \grad_h f - f \grad_h\mathcal{H}\right] + R \\
&= \left[1 -\frac{p}{|p|}\right] A(\grad_h f) +
|p|\mathcal{H}\xi - |p| f \grad_h\mathcal{H} + R
\end{split}
\end{equation}
where $R$ satisfies,
\[
\begin{split}
g(R - |p| \Tr (\widehat{Rm}(\xi,\cdot,\cdot,\nu))) \nu, X) &= |p|\frac{1}{f} g(\Tr \left(\widehat{Rm}(\xi, \cdot, \cdot, \nu)\right)\grad_h f, X) - |p| g(\grad_h \Tr \left(\widehat{Rm}(\xi, \cdot, \cdot, \nu)\right), X) \\
&\quad + \frac{p}{|p|f} \left[\langle \widehat{Rm}(\xi,\grad_h f)X,\nu\rangle -
\Tr (\widehat{Rm}(\xi,\cdot,\cdot,\nu))g(\grad_h f, X)\right] \\
&\quad  -\frac{p}{|p|} \left[\widehat{Rm}(X, \grad_h f)\xi\right]^{\xi}.
\end{split}
\]
\end{proof}

For the purpose of obtaining a Harnack inequality, the main ingredient turns out to be the evolution of the affine mean curvature $\mathcal{H}$.

\begin{theorem} We have
\begin{align*}
\partial_t\mathcal{H}= |p| \Delta \mathcal{H}+\frac{p}{|p|}| A |^2+ |p|  \mathcal{H}^2+ |p|  g^{lk}\partial_l\mathcal{H} \Tr_{12}( C _{ijk}).
\end{align*}
\end{theorem}
\begin{proof}
We will first calculate the evolution equation of $ A _{ij}.$ Recall that $$\partial_i\xi=- A _i^k\partial_kF.$$ Thus
\begin{align*}
\frac{p}{|p|}\left(- p  g^{ij}\partial_i\mathcal{H}\partial_jF+ p  \mathcal{H}\xi\right)_i&=\partial_t\xi_i=-(\partial_t A _i^k)\partial_kF+\frac{p}{|p|} A _i^k A _j^k\partial_jF.
\end{align*}
We calculate
\begin{align*}
\partial_t A _i^k=\frac{p}{|p|}( A _i^m A _m^k+ p  \mathcal{H}_{;mi}g^{mk}+ p
g^{nm}\partial_n \mathcal{H} C _{mi}^k+ p  \mathcal{H} A _i^k).
\end{align*}
Therefore,
\begin{align*}
\partial_t A _{ij}&=\partial_t( A _i^kg_{kj})\\
&=\frac{p}{|p|}\left(\left( A _i^m A _m^k+ p  \mathcal{H}_{;mi}g^{mk}+ p
g^{nm}\partial_n \mathcal{H} C _{mi}^k+ p  \mathcal{H} A _i^k\right)g_{kj}- A _i^k
( A _{kj}+ p  \mathcal{H}g_{kj})\right).
\end{align*}
Rearranging terms gives
\[\partial_t  A _{ij}= |p|  (\mathcal{H}_{;ij}+  \partial_l\mathcal{H}  C _{ij}^l)\]
Therefore,
\begin{align*}
\partial_t\mathcal{H}&=|p|g^{ij}( \mathcal{H}_{;ij}+  \partial_l \mathcal{H} C ^l_{ij})+\frac{p}{|p|}( A ^{ij}+ p  \mathcal{H}g^{ij}) A _{ij}\\
&= |p| \Delta \mathcal{H}+\frac{p}{|p|}| A |^2+ |p|  \mathcal{H}^2+ |p|  g^{lk}\partial_l\mathcal{H} \Tr_{12}( C _{ijk}).
\end{align*}
\end{proof}

\section{The Harnack Inequality}

\begin{theorem}
\[\left\{
  \begin{array}{ll}
    \partial_t \left(\varphi(\nu)K^pt^{\frac{n p }{n p +1}}\right)> 0, & p>0; \\
    \partial_t \left(\varphi(\nu)K^pt^{\frac{n |p| }{n |p| -1}}\right)<0, & -\frac{1}{n}<p<0.
  \end{array}
\right.
\]
\end{theorem}
\begin{proof}
Suppose $p>0.$
By Lemma 1 we have
\begin{align*}
\partial_t \left(ft^{\frac{n p }{n p +1}}\right)&= p  t^{\frac{n p }{n p +1}-1}f\left(t\mathcal{H}+\frac{n}{n p +1}\right).
\end{align*}
Thus it suffices to show that $Q:=t\mathcal{H}+\frac{n}{n p +1}$ is always positive:
\begin{align*}
\partial_t Q&= p\Delta Q+ p  g^{lk}\partial_lQ \Tr_{12}( C _{ijk})+\mathcal{H}+t| A |^2+  tp \mathcal{H}^2\\
&\geq  p \Delta Q+ p  g^{lk}\partial_lQ \Tr_{12}( C _{ijk})+\mathcal{H}+t\frac{n p +1}{n} \mathcal{H}^2\\
&= p \Delta Q+ p  g^{lk}\partial_lQ \Tr_{12}( C _{ijk})+\frac{n p +1}{n}\mathcal{H}Q.
\end{align*}
Therefore, by the maximum principle, $Q$ is always positive.


Suppose $-\frac{1}{n}<p<0.$ We have
\begin{align*}
\partial_t \left(ft^{\frac{n |p| }{n |p| -1}}\right)&= |p|  t^{\frac{n |p| }{n |p| -1}-1}f\left(t\mathcal{H}+\frac{n}{n |p| -1}\right).
\end{align*}
Thus it suffices to show that $Q:=t\mathcal{H}+\frac{n}{n |p| -1}$ is always negative:
\begin{align*}
\partial_t Q&= |p| \Delta Q+ |p|  g^{lk}\partial_lQ \Tr_{12}( C _{ijk})+\mathcal{H}-t| A |^2+ |p|  t \mathcal{H}^2\\
&\leq  |p| \Delta Q+ |p|  g^{lk}\partial_lQ \Tr_{12}( C _{ijk})+\mathcal{H}+\frac{n |p| -1}{n}t \mathcal{H}^2\\
&= |p| \Delta Q+ |p|  g^{lk}\partial_lQ \Tr_{12}( C _{ijk})+\frac{n |p| -1}{n}\mathcal{H}Q.
\end{align*}
Therefore, by the maximum principle, $Q$ is negative positive.
\end{proof}

To get the usual Harnack estimate, we note if we define a time-dependent diffeomorphism $\varphi: M^n\to M^n$ by
\begin{align}
\partial_t\varphi^k=h^{kl}\partial_l K^{ p },
\end{align}
then $\bar{F}(x,t):=F(\varphi(x,t),t):M^{n}\to R^{n+1}$ satisfies
\begin{align}
\partial_t\bar{F}=\bar{K}^{ p }\nu,
\end{align}
where $\bar{K}(x,t):=K(\varphi(x,t),t)$. So we have
\begin{align}
\partial_t\bar{K}^{ p }-h^{kl}\partial_k\bar{K}^{ p }\partial_l\bar{K}^{ p }+\frac{n p }{(n p +1)t}\geq 0.
\end{align}

\bibliographystyle{amsplain}
\bibliography{Bibliography.bib}

\end{document}
